LinearScan/NonEmpty0.hs
@@ -2,6 +2,7 @@ module LinearScan.NonEmpty0 where
 
 
 import qualified Prelude
+import qualified Data.IntMap
 import qualified Data.List
 import qualified Data.Ord
 import qualified Data.Functor.Identity
