LinearScan/ssrfun.hs
@@ -2,6 +2,7 @@ module LinearScan.Ssrfun where
 
 
 import qualified Prelude
+import qualified Data.IntMap
 import qualified Data.List
 import qualified Data.Ord
 import qualified Data.Functor.Identity
