Blocks.v
@@ -16,49 +16,51 @@ Section Blocks.
 
 Open Scope program_scope.
 
+Variables accType    : Set.
 Variables blockType1 : Set.
 Variables blockType2 : Set.
 Variables opType1    : Set.
 Variables opType2    : Set.
 Variables varType    : Set.
 
-Inductive VarKind := Input | Temp | Output.
+Inductive VarKind : Set := Input | Temp | Output.
 
-(* When use of a variable is encountered, one or more actions should be taken: *)
-Inductive VarAction := Spill | Restore | RestoreAndSpill.
+Definition VarId := nat.
 
 (* [VarInfo] abstracts information about the caller's notion of variables
    associated with an operation. *)
 Record VarInfo (varType : Set) := {
-  varId       : varType -> nat;     (* from 0 to highest var index *)
+  varId       : varType -> VarId;     (* from 0 to highest var index *)
   varKind     : varType -> VarKind;
   regRequired : varType -> bool
 }.
 
 Variable vinfo : VarInfo varType.
 
-Inductive OpKind := Normal | LoopBegin | LoopEnd | Call.
-
-Record AllocInfo := {
-  allocReg    : PhysReg;
-  allocAction : option VarAction
-}.
+Inductive OpKind : Set :=
+  IsNormal | IsCall | IsBranch | IsLoopBegin | IsLoopEnd.
 
 (* The [OpInfo] structure is a collection of functions that allow us to
    determine information about each operation coming from the caller's
    side. *)
-Record OpInfo (opType1 opType2 varType : Set) := {
+Record OpInfo (accType opType1 opType2 varType : Set) := {
   opKind      : opType1 -> OpKind;
   opRefs      : opType1 -> seq varType * seq PhysReg;
-  applyAllocs : forall a, opType1 -> a -> seq (nat * AllocInfo)
-                  -> a * seq opType2
+  saveOp      : VarId -> opType2;
+  restoreOp   : VarId -> opType2;
+  applyAllocs : opType1 -> accType -> seq (VarId * PhysReg)
+                  -> accType * opType2
 }.
 
-Variable oinfo : OpInfo opType1 opType2 varType.
+Variable oinfo : OpInfo accType opType1 opType2 varType.
+
+Definition BlockId := nat.
 
 Record BlockInfo (blockType1 blockType2 opType1 opType2 : Set) := {
-  blockOps    : blockType1 -> seq opType1;
-  setBlockOps : blockType1 -> seq opType2 -> blockType2
+  blockId         : blockType1 -> BlockId;
+  blockSuccessors : blockType1 -> seq BlockId;
+  blockOps        : blockType1 -> seq opType1;
+  setBlockOps     : blockType1 -> seq opType2 -> blockType2
 }.
 
 Variable binfo : BlockInfo blockType1 blockType2 opType1 opType2.
@@ -180,17 +182,157 @@ Definition numberOperations : BlockState unit := return_ tt.
   (*           ; regRefs := regRefs op |}) in *)
   (* imodify SSError (@snd _ _ \o mapAccumLOps f 1). *)
 
-(* jww (2014-12-01): The following two functions are used for computing
-   accurate live ranges. they constitute a dataflow analysis which determines
-   the true live range for variables referenced from loops.  At the moment
-   these are being left unimplemented, but this is very likely something that
-   will need to be done for the sake of the correctness of the algorithm. *)
-Definition computeLocalLiveSets : BlockState unit := return_ tt.
+Definition OpId := nat.
 
-Definition computeGlobalLiveSets : BlockState unit := return_ tt.
+Record BlockLiveSets := {
+  blockLiveGen   : seq VarId;
+  blockLiveKill  : seq VarId;
+  blockLiveIn    : seq VarId;
+  blockLiveOut   : seq VarId;
+  blockFirstOpId : OpId;
+  blockLastOpId  : OpId
+}.
+
+Section IntMap.
+
+Variable a : Type.
+
+Inductive IntMap :=
+  | emptyIntMap
+  | getIntMap of seq (nat * a).
+
+Definition IntMap_lookup (key : nat) (m : IntMap) : option a.
+Admitted.
+
+Definition IntMap_insert (key : nat) (value : a) (m : IntMap) : IntMap.
+Admitted.
+
+Definition IntMap_alter (f : option a -> option a) (key : nat) (m : IntMap) :
+  IntMap.
+Admitted.
+
+End IntMap.
+
+Definition union (a : eqType) (m1 m2 : seq a) : seq a := undup (m1 ++ m2).
+
+Definition relative_complement (a : eqType) (m1 m2 : seq a) : seq a :=
+  [seq i <- m1 | i \notin m2].
+
+Arguments emptyIntMap [a].
+Arguments getIntMap [a] _.
+
+Definition forFold {A B : Type} (b : B) (v : seq A) (f : B -> A -> B) : B :=
+  foldl f b v.
+
+Definition computeLocalLiveSets (blocks : BlockList) : IntMap BlockLiveSets :=
+  (* for each block b in blocks do
+       b.live_gen  = { }
+       b.live_kill = { }
+
+       for each operation op in b.operations do
+         visitor.visit(op)
+
+         for each virtual register opr in visitor.input_oprs do
+           if opr ∉ block.live_kill then
+             b.live_gen = b.live_gen ∪ { opr }
+         end for
+
+         for each virtual register opr in visitor.temp_oprs do
+           b.live_kill = b.live_kill ∪ { opr }
+         end for
+
+         for each virtual register opr in visitor.output_oprs do
+           b.live_kill = b.live_kill ∪ { opr }
+         end for
+       end for
+     end for *)
+  @snd _ _ $
+  forFold (1, emptyIntMap) blocks $ fun acc b => let: (idx, m) := acc in
+    let liveSet :=
+        {| blockLiveGen   := [::]
+         ; blockLiveKill  := [::]
+         ; blockLiveIn    := [::]
+         ; blockLiveOut   := [::]
+         ; blockFirstOpId := idx
+         ; blockLastOpId  := idx
+         |} in
+    let: (lastIdx', liveSet3) :=
+      forFold (idx, liveSet) (blockOps binfo b) $ fun acc o =>
+        let: (lastIdx, liveSet1) := acc in
+        (lastIdx.+2,
+         forFold liveSet1 (fst (opRefs oinfo o)) $ fun liveSet2 v =>
+           let vid := varId vinfo v in
+           if varKind vinfo v is Input
+           then
+             if vid \notin blockLiveKill liveSet2
+             then {| blockLiveGen   := vid :: blockLiveGen liveSet2
+                   ; blockLiveKill  := blockLiveKill liveSet2
+                   ; blockLiveIn    := blockLiveIn liveSet2
+                   ; blockLiveOut   := blockLiveOut liveSet2
+                   ; blockFirstOpId := blockFirstOpId liveSet2
+                   ; blockLastOpId  := lastIdx
+                   |}
+             else liveSet2
+           else
+             {| blockLiveGen   := blockLiveGen liveSet2
+              ; blockLiveKill  := vid :: blockLiveKill liveSet2
+              ; blockLiveIn    := blockLiveIn liveSet2
+              ; blockLiveOut   := blockLiveOut liveSet2
+              ; blockFirstOpId := blockFirstOpId liveSet2
+              ; blockLastOpId  := lastIdx
+              |})
+      in
+    (lastIdx', IntMap_insert (blockId binfo b) liveSet3 m).
+
+Definition computeGlobalLiveSets (blocks : BlockList)
+  (liveSets : IntMap BlockLiveSets) : IntMap BlockLiveSets :=
+  (* do
+       for each block b in blocks in reverse order do
+         b.live_out = { }
+         for each successor sux of b do
+           b.live_out = b.live_out ∪ sux.live_in
+         end for
+
+         b.live_in = (b.live_out – b.live_kill) ∪ b.live_gen
+       end for
+     while change occurred in any live set *)
+  forFold liveSets (rev blocks) $ fun liveSets1 b =>
+    let bid := blockId binfo b in
+    match IntMap_lookup bid liveSets1 with
+    | None => liveSets1         (* should never happen *)
+    | Some liveSet =>
+      let liveSet2 :=
+        forFold liveSet (blockSuccessors binfo b) $ fun liveSet1 s_bid =>
+          match IntMap_lookup s_bid liveSets1 with
+          | None => liveSet1  (* should never happen *)
+          | Some sux =>
+            {| blockLiveGen   := blockLiveGen liveSet1
+             ; blockLiveKill  := blockLiveKill liveSet1
+             ; blockLiveIn    := blockLiveIn liveSet1
+             ; blockLiveOut   := union (blockLiveOut liveSet1)
+                                       (blockLiveIn sux)
+             ; blockFirstOpId := blockFirstOpId liveSet1
+             ; blockLastOpId  := blockLastOpId liveSet1
+             |}
+          end
+        in
+      IntMap_insert bid
+        {| blockLiveGen   := blockLiveGen liveSet2
+         ; blockLiveKill  := blockLiveKill liveSet2
+         ; blockLiveIn    :=
+             union (relative_complement (blockLiveOut liveSet2)
+                                        (blockLiveKill liveSet2))
+                   (blockLiveGen liveSet2)
+         ; blockLiveOut   := blockLiveOut liveSet2
+         ; blockFirstOpId := blockFirstOpId liveSet2
+         ; blockLastOpId  := blockLastOpId liveSet2
+         |} liveSets1
+    end.
 
 Definition buildIntervals : BlockState (ScanStateSig InUse) :=
-  let mkint (vid : nat)
+  (* jww (2015-01-27): NYI: Still need to insert length-1 fixed intervals at
+     call points. *)
+  let mkint (vid : VarId)
             (ss : ScanStateSig Pending)
             (pos : nat)
             (mx : option (BoundedRange pos.*2.+1))
@@ -223,74 +365,203 @@ Definition buildIntervals : BlockState (ScanStateSig InUse) :=
      return_ s5)
   (processOperations blocks).
 
-Definition resolveDataFlow : BlockState unit := return_ tt.
+Inductive InsertPos : Set := AtBegin of VarId | AtEnd of VarId.
 
-(* Definition mapOps (f : opType -> opType) : BlockList -> BlockList := *)
-(*   NE_map (fun blk => setBlockOps binfo blk (map f (blockOps binfo blk))). *)
+Section EqInsertPos.
+
+Definition eqact v1 v2 :=
+  match v1, v2 with
+  | AtBegin r1, AtBegin r2 => r1 == r2
+  | AtEnd r1,   AtEnd r2   => r1 == r2
+  | _, _ => false
+  end.
+
+Lemma eqactP : Equality.axiom eqact.
+Proof.
+  move.
+  case=> [r1|r1];
+  case=> [r2|r2];
+  case: (r1 =P r2) => [<-|/eqP /negbTE neqx] //=;
+    do [ rewrite eq_refl;
+         by constructor
+       | rewrite neqx;
+         constructor;
+         move/eqP in neqx;
+         move=> H;
+         contradiction neqx;
+         congruence
+       | constructor;
+         discriminate
+       | idtac ].
+Qed.
+
+Canonical act_eqMixin := EqMixin eqactP.
+Canonical act_eqType := Eval hnf in EqType InsertPos act_eqMixin.
+
+Lemma eqactE : eqact = eq_op. Proof. by []. Qed.
+
+Definition InsertPos_eqType (A : eqType) :=
+  Equality.Pack act_eqMixin InsertPos.
+
+End EqInsertPos.
+
+Definition resolveDataFlow `(st : ScanState InUse sd)
+  (blocks : BlockList) (liveSets : IntMap BlockLiveSets) :
+  IntMap (seq InsertPos) :=
+  (* for each block from in blocks do
+       for each successor to of from do
+         // collect all resolving moves necessary between the blocks from
+         // and to
+         for each operand opr in to.live_in do
+           Interval parent_interval = intervals[opr]
+
+           Interval from_interval = parent_interval.child_at(from.last_op.id)
+           Interval to_interval = parent_interval.child_at(to.first_op.id)
+
+           if from_interval ≠ to_interval then
+             // interval was split at the edge between the blocks from and to
+             resolver.add_mapping(from_interval, to_interval)
+           end if
+         end for
+
+         // the moves are inserted either at the end of block from or at the
+         // beginning of block to, depending on the control flow
+         resolver.find_insert_position(from, to)
+
+         // insert all moves in correct order (without overwriting registers
+         // that are used later)
+         resolver.resolve_mappings()
+       end for
+     end for *)
+  forFold emptyIntMap blocks $ fun mappings b =>
+    let bid := blockId binfo b in
+    match IntMap_lookup bid liveSets with
+    | None => mappings
+    | Some from =>
+      (fun successors =>
+        forFold mappings successors $ fun ms s_bid =>
+          match IntMap_lookup s_bid liveSets with
+          | None => ms
+          | Some to =>
+            forFold ms (blockLiveIn to) $ fun ms' vid =>
+              if lookupInterval st vid (blockLastOpId from)
+                 is Some from_interval
+              then
+                if lookupInterval st vid (blockFirstOpId to)
+                   is Some to_interval
+                then
+                  if from_interval != to_interval
+                  then
+                    let in_from := size successors <= 1 in
+                    let ins     := if in_from
+                                   then AtEnd vid
+                                   else AtBegin vid in
+                    let f mxs   := if mxs is Some xs
+                                   then if ins \notin xs
+                                        then Some (ins :: xs)
+                                        else Some xs
+                                   else Some [:: ins] in
+                    let key     := if in_from
+                                   then bid
+                                   else s_bid in
+                    IntMap_alter f key ms'
+                  else ms'    (* should be impossible *)
+                else ms'      (* should be impossible *)
+              else ms'        (* should be impossible *)
+          end)
+      (blockSuccessors binfo b)
+    end.
 
 Section Allocation.
 
-Variable accType : Set.
-
 Record AssnStateInfo := {
-  assnOpId : nat;
+  assnOpId : OpId;
   assnAcc  : accType
 }.
 
 Definition AssnState :=
   IState SSError AssnStateInfo AssnStateInfo.
 
-Definition concatMapOpsM (f : opType1 -> AssnState (seq opType2)) :=
-  mapM (fun blk => setBlockOps binfo blk
-                     <$$> concatMapM f (blockOps binfo blk)).
+Definition savesAndRestores (opid : OpId) (vid : VarId)
+  (int : IntervalDesc) : (seq opType2 * seq opType2) :=
+  let isFirst := firstUsePos int == opid in
+  let isLast  := nextUseAfter int opid == None in
+  let save := [:: saveOp oinfo vid] in
+  let restore := [:: restoreOp oinfo vid] in
+  match iknd int, isFirst, isLast with
+  | Middle,    true,  true  => (restore, save)
+  | Middle,    false, true  => ([::], save)
+  | Middle,    true,  false => (restore, [::])
+  | LeftMost,  _,     true  => ([::], save)
+  | RightMost, true,  _     => (restore, [::])
+  | _,         _,     _     => ([::], [::])
+  end.
 
-Definition allocVar (vid : nat) (int : IntervalDesc) (reg : PhysReg) :
-  AssnState (nat * AllocInfo) :=
+Definition doAllocations (ints : seq (IntervalDesc * PhysReg))
+  (op : opType1) : AssnState (seq opType2) :=
   assn <<- iget SSError ;;
-  let n := assnOpId assn in
-  let isFirst := firstUsePos int == n in
-  let isLast  := nextUseAfter int n == None in
-  let action :=
-    match iknd int, isFirst, isLast with
-    | Middle,    true,  true  => Some RestoreAndSpill
-    | Middle,    false, true  => Some Spill
-    | Middle,    true,  false => Some Restore
-    | LeftMost,  _,     true  => Some Spill
-    | RightMost, true,  _     => Some Restore
-    | _,         _,     _     => None
-    end in
-  return_ (vid, {| allocReg    := reg
-                 ; allocAction := action |}).
-
-Definition isWithin (vid opid : nat) (int : IntervalDesc) : bool :=
-  (ivar int == vid) && (ibeg int <= opid < iend int).
-
-Definition getAllocations (ints : seq (IntervalDesc * PhysReg))
-  (v : varType) : AssnState (seq (nat * AllocInfo)) :=
-  assn <<- iget SSError ;;
-  let vid := varId vinfo v in
-  mapM (uncurry (allocVar vid))
-       [seq x <- ints | isWithin vid (assnOpId assn) (fst x)].
-
-Definition considerOp (ints : seq (IntervalDesc * PhysReg)) (op : opType1) :
-  AssnState (seq opType2) :=
-  vars <<- concatMapM (getAllocations ints) (fst (opRefs oinfo op)) ;;
+  let opid := assnOpId assn in
+  let vars := fst (opRefs oinfo op) in
+  let: (allocs, restores, saves) :=
+    forFold ([::], [::], [::]) vars $ fun acc v =>
+      let vid := varId vinfo v in
+      let v_ints :=
+          [seq x <- ints | isWithin (fst x) vid (assnOpId assn)] in
+      forFold acc v_ints $ fun acc' ir =>
+        let: (int, reg) := ir in
+        let: (allocs', restores', saves') := acc' in
+        let: (ss, rs) := savesAndRestores opid vid int in
+        ((vid, reg) :: allocs', rs ++ restores', ss ++ saves') in
+  let: (acc', op') := applyAllocs oinfo op (assnAcc assn) allocs in
   (* With lenses, this would just be: assnOpId += 2 *)
-  assn <<- iget SSError ;;
-  let: (acc', op') := applyAllocs oinfo op (assnAcc assn) vars in
-  iput SSError
-       {| assnOpId := (assnOpId assn).+2
-        ; assnAcc  := acc' |} ;;;
-  return_ op'.
+  iput SSError {| assnOpId := (assnOpId assn).+2
+                ; assnAcc  := acc' |} ;;;
+  return_ $ restores ++ op' :: saves.
 
-Definition assignRegNum `(st : ScanState InUse sd) (acc : accType) :
+Definition considerOps (f : opType1 -> AssnState (seq opType2))
+  (mappings : IntMap (seq InsertPos)) :=
+  mapM $ fun blk =>
+    (* First apply all allocations *)
+    let ops := blockOps binfo blk in
+    ops' <<- concatMapM f ops ;;
+    (* Insert resolving moves based on the mappings *)
+    let bid := blockId binfo blk in
+    let ops'' :=
+        if IntMap_lookup bid mappings is Some inss
+        then forFold ops' inss $ fun ops'' ins =>
+          (* jww (2015-01-27): NYI: When multiple moves must be inserted at
+             one edge, then the order of the moves is important because the
+             same register can occur as the source of one move and the
+             destination of another move. The moves must be ordered such that
+             a register is saved first before it is overwritten. *)
+          match ins with
+          | AtBegin vid => restoreOp oinfo vid :: ops''
+          | AtEnd   vid =>
+            (fun sop =>
+              if ops is o :: os
+              then
+                if ops'' is o'' :: os''
+                then
+                  if opKind oinfo (last o os) is IsBranch
+                  then belast o'' os'' ++ [:: sop; last o'' os'']
+                  else ops' ++ [:: sop]
+                else [:: sop]
+              else [:: sop])
+            (saveOp oinfo vid)
+          end
+        else ops' in
+    return_ $ setBlockOps binfo blk ops''.
+
+Definition assignRegNum `(st : ScanState InUse sd)
+  (mappings : IntMap (seq InsertPos)) (acc : accType) :
   IState SSError (seq blockType1) (seq blockType2) accType :=
-  let ints := map (fun x => (getIntervalDesc (getInterval (fst x)), snd x))
-                  (handled sd ++ active sd ++ inactive sd) in
+  let ints :=
+      map (fun x => (getIntervalDesc (getInterval (fst x)), snd x))
+          (handled sd ++ active sd ++ inactive sd) in
   blocks <<- iget SSError ;;
-  match runIState SSError (concatMapOpsM (considerOp ints) blocks)
-                  {| assnOpId  := 1
-                   ; assnAcc := acc |} with
+  match (considerOps (doAllocations ints) mappings blocks)
+        {| assnOpId := 1
+         ; assnAcc := acc |} with
   | inl err => ierr SSError err
   | inr (blocks', assn) =>
       iput SSError blocks' ;;;
