fixcode.pl
@@ -5,6 +5,7 @@ while (<>) {
     s/import qualified LinearScan\.GHC/import qualified GHC/;
     s{import qualified LinearScan\.Prelude as Prelude}{
 import qualified Prelude
+import qualified Data.IntMap
 import qualified Data.List
 import qualified Data.Ord
 import qualified Data.Functor.Identity
